formula_prices_list.thy
@@ -49,7 +49,7 @@ expr_1_conj_right:\<open>expr_1 (HML_conj [] (y#ys)) = (Max ({0} \<union> {expr_
 expr_1_pos: \<open>expr_1 (HML_poss \<alpha> \<phi>) = 
   1 + (expr_1 \<phi>)\<close>
 
-(*TODO: Lemma fertig beweisen (Sorry's)*)
+(*Done*)
 lemma expr_1_set_form: "expr_1 (HML_conj \<Phi> \<Psi>) =
 Max({0} \<union> {expr_1 x | x. x \<in> set \<Phi>} \<union> {expr_1 y | y. y \<in> set \<Psi>})"
 proof(induction \<Phi>)
@@ -72,10 +72,23 @@ proof(induction \<Phi>)
       finally have expr_1_IS: "expr_1 (HML_conj [] (a#\<Psi>)) = 
 (Max ({0} \<union> {expr_1 a} \<union> {Max ({0} \<union> {expr_1 x |x. x \<in> set []} \<union> {expr_1 y |y. y \<in> set \<Psi>})}))"
         by this
-      from A1 have "{Max ({0} \<union> {expr_1 x |x. x \<in> set []} \<union> {expr_1 y |y. y \<in> set \<Psi>})} =
-{Max {expr_1 y |y. y \<in> set (a # \<Psi>)}}" (*TODO*) sorry
-      then have "(Max ({0} \<union> {expr_1 a} \<union> {Max ({0} \<union> {expr_1 x |x. x \<in> set []} \<union> {expr_1 y |y. y \<in> set \<Psi>})})) =
- (Max ({0} \<union> {expr_1 x |x. x \<in> set []} \<union> {expr_1 y |y. y \<in> set (a # \<Psi>)}))" sorry (*TODO*)
+      have fin: "finite ({0} \<union> {expr_1 x |x. x \<in> set []} \<union> {expr_1 y |y. y \<in> set \<Psi>})"
+        by simp
+      have ne: "({0} \<union> {expr_1 x |x. x \<in> set []} \<union> {expr_1 y |y. y \<in> set \<Psi>}) \<noteq> {}"
+        by simp
+      have "\<forall>x \<in> {0} \<union> {expr_1 x |x. x \<in> set []} \<union> {expr_1 y |y. y \<in> set \<Psi>}. x \<le>
+Max({0} \<union> {expr_1 x |x. x \<in> set []} \<union> {expr_1 y |y. y \<in> set \<Psi>})"
+        by simp
+      thm Max_in
+      from fin ne have "Max({0} \<union> {expr_1 x |x. x \<in> set []} \<union> {expr_1 y |y. y \<in> set \<Psi>}) \<in> 
+{0} \<union> {expr_1 x |x. x \<in> set []} \<union> {expr_1 y |y. y \<in> set \<Psi>}"
+        by (smt (verit, best) Max_in emptyE empty_Collect_eq empty_set)
+      then have "(Max ({0} \<union> {expr_1 a} \<union> {Max ({0} \<union> {expr_1 x |x. x \<in> set []} \<union> {expr_1 y |y. y \<in> set \<Psi>})})) = 
+(Max ({0} \<union> {expr_1 a} \<union> {0} \<union> {expr_1 x |x. x \<in> set []} \<union> {expr_1 y |y. y \<in> set \<Psi>}))" 
+        by simp
+      also from A1 have "(Max ({0} \<union> {expr_1 a} \<union> {0} \<union> {expr_1 x |x. x \<in> set []} \<union> {expr_1 y |y. y \<in> set \<Psi>})) = 
+Max ({0} \<union> {expr_1 y |y. y \<in> set (a # \<Psi>)} \<union> {0} \<union> {expr_1 x |x. x \<in> set []})"
+        by simp
       from this expr_1_IS show ?thesis by simp
     qed
   qed
@@ -91,11 +104,33 @@ next
       also have "... = 
 (Max ({0} \<union> {expr_1 a} \<union> {Max ({0} \<union> {expr_1 x |x. x \<in> set \<Phi>} \<union> {expr_1 y |y. y \<in> set []})}))"
         using local.Nil by force
-      finally have "expr_1 (HML_conj (a#\<Phi>) []) = 
+      finally have expr_1_eq: "expr_1 (HML_conj (a#\<Phi>) []) = 
 (Max ({0} \<union> {expr_1 a} \<union> {Max ({0} \<union> {expr_1 x |x. x \<in> set \<Phi>} \<union> {expr_1 y |y. y \<in> set []})}))"
         by this
-      then show "expr_1 (HML_conj (a#\<Phi>) []) = 
-(Max ({0} \<union> {expr_1 x |x. x \<in> set (a # \<Phi>)} \<union> {expr_1 y |y. y \<in> set []}))" sorry (*TODO*)
+      have ne: "{0} \<union> {expr_1 x |x. x \<in> set \<Phi>} \<union> {expr_1 y |y. y \<in> set []} \<noteq> {}"
+        by simp
+      have fin: "finite ({0} \<union> {expr_1 x |x. x \<in> set \<Phi>} \<union> {expr_1 y |y. y \<in> set []})"
+        by simp
+      have fa: "\<forall>x \<in> {0} \<union> {expr_1 x |x. x \<in> set \<Phi>} \<union> {expr_1 y |y. y \<in> set []}. x \<le>
+Max({0} \<union> {expr_1 x |x. x \<in> set \<Phi>} \<union> {expr_1 y |y. y \<in> set []})"
+        by simp
+      from fin ne have "Max({0} \<union> {expr_1 x |x. x \<in> set \<Phi>} \<union> {expr_1 y |y. y \<in> set []}) \<in>
+{0} \<union> {expr_1 x |x. x \<in> set \<Phi>} \<union> {expr_1 y |y. y \<in> set []}" 
+        by (smt (verit, best) Max_in emptyE empty_Collect_eq empty_set)
+      from this fa have "(Max ({0} \<union> {expr_1 a} \<union> {Max ({0} \<union> {expr_1 x |x. x \<in> set \<Phi>} \<union> {expr_1 y |y. y \<in> set []})})) = 
+(Max ({0} \<union> {expr_1 a} \<union> {0} \<union> {expr_1 x |x. x \<in> set \<Phi>} \<union> {expr_1 y |y. y \<in> set []}))" 
+        by simp
+      also have eq2: "(Max ({0} \<union> {expr_1 a} \<union> {0} \<union> {expr_1 x |x. x \<in> set \<Phi>} \<union> {expr_1 y |y. y \<in> set []})) = 
+(Max ({0} \<union> {expr_1 a}  \<union> {expr_1 x |x. x \<in> set \<Phi>} \<union> {expr_1 y |y. y \<in> set []}))"
+        by simp
+      have "{expr_1 a}  \<union> {expr_1 x |x. x \<in> set \<Phi>} = {expr_1 x |x. x \<in> set (a#\<Phi>)}"
+        by auto
+      then have "(Max ({0} \<union> {expr_1 a}  \<union> {expr_1 x |x. x \<in> set \<Phi>} \<union> {expr_1 y |y. y \<in> set []})) = 
+(Max ({0}  \<union> {expr_1 x |x. x \<in> set (a#\<Phi>)} \<union> {expr_1 y |y. y \<in> set []}))"
+        by (metis (mono_tags, lifting) eq2 sup_assoc)
+      from this expr_1_eq show "expr_1 (HML_conj (a#\<Phi>) []) = 
+(Max ({0} \<union> {expr_1 x |x. x \<in> set (a # \<Phi>)} \<union> {expr_1 y |y. y \<in> set []}))" 
+        by simp
     qed
   next
     case (Cons b \<Psi>)
@@ -103,14 +138,25 @@ next
     proof-
       have A1: "{expr_1 a} \<union> {expr_1 x |x. x \<in> set \<Phi>} = {expr_1 x |x. x \<in> set (a # \<Phi>)}" 
         by auto
+      have ne: "{0} \<union> {expr_1 x |x. x \<in> set \<Phi>} \<union> {expr_1 y |y. y \<in> set (b # \<Psi>)} \<noteq> {}"
+        by simp
+      have fin: "finite ({0} \<union> {expr_1 x |x. x \<in> set \<Phi>} \<union> {expr_1 y |y. y \<in> set (b # \<Psi>)})"
+        by simp
+      have fa: "\<forall>x \<in> ({0} \<union> {expr_1 x |x. x \<in> set \<Phi>} \<union> {expr_1 y |y. y \<in> set (b # \<Psi>)}). x \<le>
+Max ({0} \<union> {expr_1 x |x. x \<in> set \<Phi>} \<union> {expr_1 y |y. y \<in> set (b # \<Psi>)})" 
+        by simp
+      from fin ne have elem: "Max ({0} \<union> {expr_1 x |x. x \<in> set \<Phi>} \<union> {expr_1 y |y. y \<in> set (b # \<Psi>)}) \<in>
+({0} \<union> {expr_1 x |x. x \<in> set \<Phi>} \<union> {expr_1 y |y. y \<in> set (b # \<Psi>)})"
+        by (smt (verit, best) Max_in emptyE empty_Collect_eq empty_set)
       have "expr_1 (HML_conj (a # \<Phi>) (b # \<Psi>)) = 
 (Max ({0} \<union> {expr_1 a} \<union> {expr_1 (HML_conj \<Phi> (b#\<Psi>))}))"
         by simp
       also have "... = 
 (Max ({0} \<union> {expr_1 a} \<union> {Max ({0} \<union> {expr_1 x |x. x \<in> set \<Phi>} \<union> {expr_1 y |y. y \<in> set (b # \<Psi>)})}))"
         using Cons.prems by presburger
-      also have "... = 
-(Max ({0} \<union> {expr_1 a} \<union> {expr_1 x |x. x \<in> set \<Phi>} \<union> {expr_1 y |y. y \<in> set (b # \<Psi>)}))" sorry
+      also from fa elem have "... = 
+(Max ({0} \<union> {expr_1 a} \<union> {expr_1 x |x. x \<in> set \<Phi>} \<union> {expr_1 y |y. y \<in> set (b # \<Psi>)}))" 
+        by simp
       also from A1 have "... = Max ({0} \<union> {expr_1 x |x. x \<in> set (a # \<Phi>)} \<union> {expr_1 y |y. y \<in> set (b # \<Psi>)})"
         by (metis (no_types, lifting) sup_assoc)
       finally show "expr_1 (HML_conj (a # \<Phi>) (b # \<Psi>)) = 
@@ -133,7 +179,10 @@ expr_2_conj: \<open>expr_2 (HML_conj (x#xs) \<Psi>) = (Max ({1 + expr_2 x} \<uni
 expr_2_conj_right:\<open>expr_2 (HML_conj [] (y#ys)) = (Max ({1 + expr_2 y} \<union> {expr_2 (HML_conj [] ys)}))\<close> |
 expr_2_pos: \<open>expr_2 (HML_poss \<alpha> \<phi>) = expr_2 \<phi>\<close>
 
-(*Für formula_list Definition: Menge Pos ist \<Phi>, Menge Ng ist \<Phi>.?!*)
+(*TODO*)
+lemma expr_2_set: "expr_2 (HML_conj \<Phi> \<Psi>) =
+Max({1} \<union> {1 + expr_2 x | x. x \<in> set \<Phi>} \<union> {1 + expr_2 y | y. y \<in> set \<Psi>})"
+  sorry
 
 fun pos_r :: "('a)formula_list list \<Rightarrow> ('a)formula_list list"
   where
@@ -148,7 +197,6 @@ fun r :: "('a)formula_list list \<Rightarrow> nat"
 \<open>r xs = Max (set (map(\<lambda>x. expr_1 x) xs))\<close>
 
 
-(*TODO: überprüfen*)
 fun expr_3 :: "('a) formula_list \<Rightarrow> nat"
 where
  expr_3_pos: \<open>expr_3 (HML_poss \<alpha> \<phi>) = expr_3 \<phi>\<close>
@@ -157,38 +205,177 @@ where
 | expr_3_conj: \<open>expr_3 (HML_conj (x#xs) \<Psi>) = 
 Max ({0} \<union> {expr_1 x} \<union> {expr_3 (HML_conj xs \<Psi>)} \<union> {expr_3 x})\<close>
 
+(*TODO*)
+lemma expr_3_set: "expr_3 (HML_conj \<Phi> \<Psi>) =
+Max({0} \<union> {expr_3 x | x. x \<in> set \<Phi>} \<union> {expr_3 y | y. y \<in> set \<Psi>} \<union> {expr_1 x | x. x \<in> set \<Phi>})"
+  sorry
 
 (* Neg := {i \<in> I| \<exists>\<phi>\<^sub>i. \<psi>\<^sub>i = \<not>\<phi>\<^sub>i}*)
 
-fun expr_4_rest :: "('a)formula_list \<Rightarrow> nat"
+fun 
+  expr_4 :: "('a)formula_list \<Rightarrow> nat" and
+expr_4_2 :: "('a)formula_list \<Rightarrow> ('a)formula_list list \<Rightarrow> nat"
 where
- expr_4_pos: \<open>expr_4_rest (HML_poss \<alpha> \<phi>) = expr_4_rest \<phi>\<close> |
-expr_4_conj_empty: \<open>expr_4_rest (HML_conj [] []) = 0\<close>|
-expr_4_conj_right: \<open>expr_4_rest (HML_conj [] (y#ys)) = Max ({0} \<union> {expr_4_rest y} \<union> {expr_4_rest (HML_conj [] ys)})\<close>|
-expr_4_conj: \<open>expr_4_rest (HML_conj (x#xs) \<Psi>) = 
-Max ({0} \<union> {expr_4_rest x} \<union> {expr_4_rest (HML_conj xs \<Psi>)})\<close>
+"expr_4 (HML_poss a \<phi>) = expr_4 \<phi>" |
+"expr_4 (HML_conj \<Phi> \<Psi>) = expr_4_2 (HML_conj \<Phi> \<Psi>) \<Phi>" |
+"expr_4_2 (HML_poss a \<phi>) \<Phi> = expr_4 \<phi>" |
+"expr_4_2 (HML_conj [] []) y1 = Max {expr_1 (HML_conj (pos_r y1) [])}" |
+"expr_4_2 (HML_conj (a#\<Phi>) \<Psi>) y1 = Max({expr_4 a} \<union> {expr_4_2(HML_conj \<Phi> \<Psi>) y1})" |
+"expr_4_2 (HML_conj [] (a#\<Psi>)) y1 = Max({expr_4 a} \<union> {expr_4_2(HML_conj [] \<Psi>) y1})"
 
-(*TODODODOD*)
-lemma expr_4_rest_set: "expr_4_rest (HML_conj \<Phi> \<Psi>) = 
-Max({0} \<union> {expr_4_rest x |x. x \<in> set \<Phi>} \<union> {expr_4_rest y|y. y \<in> set \<Psi>})"
-  sorry
+lemma expr_4_eq_expr_4_2: "expr_4_2(HML_conj [] \<Psi>) y1 = 
+Max({expr_4 x|x. x \<in> set \<Psi>} \<union> {expr_1 (HML_conj (pos_r y1) [])})"
+proof(induction \<Psi>)
+  case Nil
+  then show ?case by simp
 
-fun expr_4_r :: "('a)formula_list \<Rightarrow> nat"
-  where
-\<open>expr_4_r (HML_conj (x#xs) \<Psi>) = Max({expr_1 x} \<union> {expr_4_r (HML_conj xs \<Psi>)})\<close>|
-\<open>expr_4_r _ = 0\<close>
+next
+  case (Cons a \<Psi>)
+  have "expr_4_2 (HML_conj [] (a # \<Psi>)) y1 = 
+Max({expr_4 a} \<union> {expr_4_2(HML_conj [] \<Psi>) y1})"
+    by simp
+  also have "... = 
+Max({expr_4 a} \<union> {Max ({expr_4 x |x. x \<in> set \<Psi>} \<union> {expr_1 (HML_conj (pos_r y1) [])})})"
+    using local.Cons by presburger
+  finally have expr_4_2_form: "expr_4_2 (HML_conj [] (a # \<Psi>)) y1 =
+Max({expr_4 a} \<union> {Max ({expr_4 x |x. x \<in> set \<Psi>} \<union> {expr_1 (HML_conj (pos_r y1) [])})})"
+    by this
+  have ne: "({expr_4 x |x. x \<in> set \<Psi>} \<union> {expr_1 (HML_conj (pos_r y1) [])}) \<noteq> {}"
+    by simp
+  have fin: "finite ({expr_4 x |x. x \<in> set \<Psi>} \<union> {expr_1 (HML_conj (pos_r y1) [])})" 
+    by simp
+  from fin ne have elem: "Max ({expr_4 x |x. x \<in> set \<Psi>} \<union> {expr_1 (HML_conj (pos_r y1) [])}) \<in> 
+({expr_4 x |x. x \<in> set \<Psi>} \<union> {expr_1 (HML_conj (pos_r y1) [])})" 
+    by (rule Max_in)
+  from fin ne have "\<forall>x \<in> ({expr_4 x |x. x \<in> set \<Psi>} \<union> {expr_1 (HML_conj (pos_r y1) [])}). 
+x \<le> Max({expr_4 x |x. x \<in> set \<Psi>} \<union> {expr_1 (HML_conj (pos_r y1) [])})"
+    by simp
+  from this elem fin ne have "Max({expr_4 a} \<union> {Max ({expr_4 x |x. x \<in> set \<Psi>} \<union> {expr_1 (HML_conj (pos_r y1) [])})}) =
+Max({expr_4 a} \<union> ({expr_4 x |x. x \<in> set \<Psi>} \<union> {expr_1 (HML_conj (pos_r y1) [])}))"
+    by (metis (no_types, lifting) Max.union Max_singleton empty_not_insert finite.emptyI finite.insertI)
+  also have eq: "... = Max({expr_4 a} \<union> {expr_4 x |x. x \<in> set \<Psi>} \<union> {expr_1 (HML_conj (pos_r y1) [])})"
+    by simp
+  have "{expr_4 a} \<union> {expr_4 x |x. x \<in> set \<Psi>} = {expr_4 x |x. x \<in> set (a # \<Psi>)}"
+    by auto
+  then have "Max({expr_4 a} \<union> {expr_4 x |x. x \<in> set \<Psi>} \<union> {expr_1 (HML_conj (pos_r y1)[])}) =
+ Max ({expr_4 x |x. x \<in> set (a # \<Psi>)} \<union> {expr_1 (HML_conj (pos_r y1) [])})"
+    by simp
+  then show ?case
+    using calculation eq expr_4_2_form by presburger
+qed
 
-lemma expr_4_r_set: "expr_4_r (HML_conj \<Phi> \<Psi>) =
-Max({0} \<union> {expr_1 x | x. x \<in> set \<Phi>})"
-  sorry
+(*Done*)
+lemma expr_4_2_eq: "expr_4_2(HML_conj \<Phi> \<Psi>) y1 =
+Max({expr_4 x|x. x\<in> set \<Phi>} \<union> {expr_4 y|y. y \<in> set \<Psi>} \<union> {expr_1 (HML_conj (pos_r y1) [])})"
+proof(induction \<Phi>)
+  case Nil
+  then show ?case
+    by (simp add: expr_4_eq_expr_4_2)
+next
+  case (Cons a \<Phi>)
+  then show ?case 
+  proof(induction \<Psi>)
+    case Nil
+    have ne: "({expr_4 x |x. x \<in> set \<Phi>} \<union> {expr_4 y |y. y \<in> set []} \<union> {expr_1 (HML_conj (pos_r y1) [])})
+\<noteq> {}"
+      by simp
+    have fin: "finite ({expr_4 x |x. x \<in> set \<Phi>} \<union> {expr_4 y |y. y \<in> set []} \<union> {expr_1 (HML_conj (pos_r y1) [])})"
+      by simp
+    from fin ne Max_in have elem: "Max({expr_4 x |x. x \<in> set \<Phi>} \<union> {expr_4 y |y. y \<in> set []} \<union> {expr_1 (HML_conj (pos_r y1) [])}) \<in>
+({expr_4 x |x. x \<in> set \<Phi>} \<union> {expr_4 y |y. y \<in> set []} \<union> {expr_1 (HML_conj (pos_r y1) [])})"
+      by (smt (verit, ccfv_threshold) emptyE empty_Collect_eq empty_set)
+    from fin ne have "\<forall>x \<in> ({expr_4 x |x. x \<in> set \<Phi>} \<union> {expr_4 y |y. y \<in> set []} \<union> {expr_1 (HML_conj (pos_r y1) [])}).
+x \<le> Max ({expr_4 x |x. x \<in> set \<Phi>} \<union> {expr_4 y |y. y \<in> set []} \<union> {expr_1 (HML_conj (pos_r y1) [])})"
+      by simp
+    from this elem fin ne have max_decompos: "Max ({expr_4 a} \<union> 
+{Max ({expr_4 x |x. x \<in> set \<Phi>} \<union> {expr_4 y |y. y \<in> set []} \<union> {expr_1 (HML_conj (pos_r y1) [])})}) =
+Max({expr_4 a} \<union> 
+({expr_4 x |x. x \<in> set \<Phi>} \<union> {expr_4 y |y. y \<in> set []} \<union> {expr_1 (HML_conj (pos_r y1) [])}))"
+      by (smt (verit, best) Max_eqI Max_singleton Sup_fin.union Sup_fin_Max empty_not_insert finite.emptyI finite.insertI)
+    have "expr_4_2 (HML_conj (a # \<Phi>) []) y1 =
+Max ({expr_4 a} \<union> {expr_4_2(HML_conj \<Phi> []) y1})"
+      by simp
+    also have eq_1: "... = 
+Max ({expr_4 a} \<union> 
+{Max ({expr_4 x |x. x \<in> set \<Phi>} \<union> {expr_4 y |y. y \<in> set []} \<union> {expr_1 (HML_conj (pos_r y1) [])})})"
+      using local.Nil by fastforce
+    finally have "expr_4_2 (HML_conj (a # \<Phi>) []) y1 =
+Max ({expr_4 a} \<union> 
+{Max ({expr_4 x |x. x \<in> set \<Phi>} \<union> {expr_4 y |y. y \<in> set []} \<union> {expr_1 (HML_conj (pos_r y1) [])})})"
+      by this
+    from max_decompos eq_1 have "expr_4_2 (HML_conj (a # \<Phi>) []) y1 = 
+Max({expr_4 a} \<union> 
+({expr_4 x |x. x \<in> set \<Phi>} \<union> {expr_4 y |y. y \<in> set []} \<union> {expr_1 (HML_conj (pos_r y1) [])}))"
+      by simp
+    then have eq: "expr_4_2 (HML_conj (a # \<Phi>) []) y1
+ = Max({expr_4 a} \<union> 
+{expr_4 x |x. x \<in> set \<Phi>} \<union> {expr_4 y |y. y \<in> set []} \<union> {expr_1 (HML_conj (pos_r y1) [])})"
+      by simp
+    have "{expr_4 a} \<union> {expr_4 x |x. x \<in> set \<Phi>} = {expr_4 x |x. x \<in> set (a#\<Phi>)}"
+      by auto
+    from this eq show ?case by simp
+  next
+    case (Cons b \<Psi>)
+    have "expr_4_2 (HML_conj (a # \<Phi>) (b # \<Psi>)) y1 = 
+Max({expr_4 a} \<union> {expr_4_2(HML_conj \<Phi> (b#\<Psi>)) y1})"
+      by simp
+    also have "... = Max({expr_4 a} \<union> 
+{Max ({expr_4 x |x. x \<in> set \<Phi>} \<union> {expr_4 y |y. y \<in> set (b # \<Psi>)} \<union> {expr_1 (HML_conj (pos_r y1) [])})})"
+      using Cons.prems by presburger
+    finally have expr_4_2_form: "expr_4_2 (HML_conj (a # \<Phi>) (b # \<Psi>)) y1 = 
+Max({expr_4 a} \<union> 
+{Max ({expr_4 x |x. x \<in> set \<Phi>} \<union> {expr_4 y |y. y \<in> set (b # \<Psi>)} \<union> {expr_1 (HML_conj (pos_r y1) [])})})"
+      by this
+    have ne:
+"({expr_4 x |x. x \<in> set \<Phi>} \<union> {expr_4 y |y. y \<in> set (b # \<Psi>)} \<union> {expr_1 (HML_conj (pos_r y1) [])}) \<noteq> 
+{}" 
+      by simp
+    have fin: 
+"finite(
+{expr_4 x |x. x \<in> set \<Phi>} \<union> {expr_4 y |y. y \<in> set (b # \<Psi>)} \<union> {expr_1 (HML_conj (pos_r y1) [])})"
+      by simp
+    from fin ne have elem: "Max ({expr_4 x |x. x \<in> set \<Phi>} \<union> {expr_4 y |y. y \<in> set (b # \<Psi>)} \<union> {expr_1 (HML_conj (pos_r y1) [])}) \<in>
+({expr_4 x |x. x \<in> set \<Phi>} \<union> {expr_4 y |y. y \<in> set (b # \<Psi>)} \<union> {expr_1 (HML_conj (pos_r y1) [])})"
+      by (rule Max_in)
+    have "\<forall>x \<in> ({expr_4 x |x. x \<in> set \<Phi>} \<union> {expr_4 y |y. y \<in> set (b # \<Psi>)} \<union> {expr_1 (HML_conj (pos_r y1) [])}). x \<le>
+Max ({expr_4 x |x. x \<in> set \<Phi>} \<union> {expr_4 y |y. y \<in> set (b # \<Psi>)} \<union> {expr_1 (HML_conj (pos_r y1) [])})"
+      by simp
+    from elem this have "Max({expr_4 a} \<union> 
+{Max ({expr_4 x |x. x \<in> set \<Phi>} \<union> {expr_4 y |y. y \<in> set (b # \<Psi>)} \<union> {expr_1 (HML_conj (pos_r y1) [])})}) =
+Max({expr_4 a} \<union> 
+({expr_4 x |x. x \<in> set \<Phi>} \<union> {expr_4 y |y. y \<in> set (b # \<Psi>)} \<union> {expr_1 (HML_conj (pos_r y1) [])}))"
+      by (metis (no_types, lifting) Max_singleton Sup_fin.union Sup_fin_Max empty_not_insert fin finite.emptyI finite.insertI ne)
+    from this expr_4_2_form have "expr_4_2 (HML_conj (a # \<Phi>) (b # \<Psi>)) y1 = 
+Max({expr_4 a} \<union> 
+({expr_4 x |x. x \<in> set \<Phi>} \<union> {expr_4 y |y. y \<in> set (b # \<Psi>)} \<union> {expr_1 (HML_conj (pos_r y1) [])}))"
+      by simp
+    also have "... = 
+Max({expr_4 a} \<union> 
+{expr_4 x |x. x \<in> set \<Phi>} \<union> {expr_4 y |y. y \<in> set (b # \<Psi>)} \<union> {expr_1 (HML_conj (pos_r y1) [])})"
+      by simp
+    finally have eq: "expr_4_2 (HML_conj (a # \<Phi>) (b # \<Psi>)) y1 =
+Max({expr_4 a} \<union> 
+{expr_4 x |x. x \<in> set \<Phi>} \<union> {expr_4 y |y. y \<in> set (b # \<Psi>)} \<union> {expr_1 (HML_conj (pos_r y1) [])})"
+      by this
+    have "{expr_4 a} \<union> {expr_4 x |x. x \<in> set \<Phi>} =  
+{expr_4 x |x. x \<in> set (a#\<Phi>)}"
+      by auto
+    from this eq show ?case by simp
+  qed
+qed
 
-
-fun expr_4 :: "('a)formula_list \<Rightarrow> nat" 
-  where
-pre_conj: \<open>expr_4 (HML_conj \<Phi> \<Psi>) = 
-Max ({expr_4_rest (HML_conj \<Phi> \<Psi>)} \<union> {expr_1 (HML_conj (pos_r \<Phi>) \<Psi>)})\<close> |
-\<open>expr_4 (HML_poss \<alpha> \<phi>) = expr_4 \<phi>\<close>
-
+(*Done*)
+lemma expr_4_set: "expr_4 (HML_conj \<Phi> \<Psi>) =
+Max ({expr_1 (HML_conj (pos_r \<Phi>)[])} \<union> {expr_4 x|x. x \<in> set \<Phi>} \<union> {expr_4 y|y. y \<in> set \<Psi>})"
+proof-
+  have "expr_4 (HML_conj \<Phi> \<Psi>) = expr_4_2 (HML_conj \<Phi> \<Psi>) \<Phi>"
+    by simp
+  also from expr_4_2_eq have "... = 
+Max ({expr_1 (HML_conj (pos_r \<Phi>)[])} \<union> {expr_4 x |x. x \<in> set \<Phi>} \<union> {expr_4 y |y. y \<in> set \<Psi>})"
+    by auto
+  finally show ?thesis
+    by this
+qed
 
 fun expr_5 :: "('a)formula_list \<Rightarrow> nat"
 where
@@ -198,6 +385,9 @@ expr_5_conj: \<open>expr_5 (HML_conj (x#xs) \<Psi>) = Max ({0} \<union> {expr_5 
 expr_5_conj_2: 
 \<open>expr_5 (HML_conj [] (y#ys)) = Max ({0} \<union> {expr_5 y} \<union> {expr_5 (HML_conj [] ys)} \<union> {expr_1 y})\<close>
 
+lemma expr_5_set: "expr_5 (HML_conj \<Phi> \<Psi>) = 
+Max({0} \<union> {expr_5 x | x. x \<in> set \<Phi>} \<union> {expr_5 y | y. y \<in> set \<Psi>} \<union> {expr_1 y | y. y \<in> set \<Psi>})"
+  sorry
 
 fun expr_6 :: "('a)formula_list \<Rightarrow> nat"
 where
@@ -205,6 +395,11 @@ expr_6_pos: \<open>expr_6 (HML_poss \<alpha> \<phi>) = expr_6 \<phi>\<close>|
 expr_6_conj_empty: \<open>expr_6 (HML_conj [] []) = 0\<close>|
 expr_6_conj: \<open>expr_6 (HML_conj (x#xs) \<Psi>) = Max({0} \<union> {expr_6 x} \<union> {expr_6 (HML_conj xs \<Psi>)})\<close> |
 expr_6_conj_2: \<open>expr_6 (HML_conj [] (y#ys)) = Max({0}  \<union> {1 + expr_6 y} \<union> {expr_6 (HML_conj [] ys)})\<close>
+
+(*TODO*)
+lemma expr_6_set: "expr_6 (HML_conj \<Phi> \<Psi>) = 
+Max({0} \<union> {expr_6 x | x. x \<in> set \<Phi>} \<union> {1 + expr_6 y | y. y \<in> set \<Psi>})"
+  sorry
 
 fun expr :: "('a)formula_list \<Rightarrow> nat \<times> nat \<times> nat \<times>  nat \<times> nat \<times> nat" 
   where
